src/Init/Prelude.lean
@@ -886,6 +886,9 @@ theorem ULift.up_down {α : Type u} (b : ULift.{v} α) : Eq (up (down b)) b := r
 /-- Bijection between `α` and `ULift.{v} α` -/
 theorem ULift.down_up {α : Type u} (a : α) : Eq (down (up.{v} a)) a := rfl
 
+instance [Inhabited α] : Inhabited (ULift α) where
+  default := ULift.up default
+
 /--
 Either a proof that `p` is true or a proof that `p` is false. This is equivalent to a `Bool` paired
 with a proof that the `Bool` is `true` if and only if `p` is true.
