src/Lean/Elab/Tactic/Do/Syntax.lean
@@ -32,17 +32,18 @@ private meta def elabTriple : TermElab
     -- then `Triple x P _` will not elaborate because `σ → Assertion ps =?= Assertion ?ps` fails.
     -- We must first instantiate `?ps` to `.arg σ ps` through the `outParam` of `WP`, hence this elaborator.
     -- This is tracked in #8766, and #8074 might be a fix.
-    let (u, m, α, ps, inst, x) ← withRef x do
+    let (u, v, m, α, ps, inst, x) ← withRef x do
       let x ← elabTerm x none
       let ty ← inferType x
       tryPostponeIfMVar ty
       let ty ← instantiateMVars ty
       let .app m α := ty.consumeMData | throwError "Type of {x} is not a type application: {ty}"
-      let some u ← Level.dec <$> getLevel ty | throwError "Wrong level 0 {ty}"
-      let ps ← mkFreshExprMVar (mkConst ``PostShape)
-      let inst ← synthInstance (mkApp2 (mkConst ``WP [u]) m ps)
-      return (u, m, α, ps, inst, x)
-    let P ← elabTerm (← `(spred($P))) (mkApp (mkConst ``Assertion) ps)
-    let Q ← elabTerm (← `(spred($Q))) (mkApp2 (mkConst ``PostCond) α ps)
-    return mkApp7 (mkConst ``Triple [u]) m ps inst α x P Q
+      let some u ← Level.dec <$> getLevel α | throwError "Wrong level 0 {ty}"
+      let some v ← Level.dec <$> getLevel ty | throwError "Wrong level 0 {ty}"
+      let ps ← mkFreshExprMVar (mkConst ``PostShape [u])
+      let inst ← synthInstance (mkApp2 (mkConst ``WP [u, v]) m ps)
+      return (u, v, m, α, ps, inst, x)
+    let P ← elabTerm (← `(spred($P))) (mkApp (mkConst ``Assertion [u]) ps)
+    let Q ← elabTerm Q (mkApp2 (mkConst ``PostCond [u]) α ps)
+    return mkApp7 (mkConst ``Triple [u, v]) m ps inst α x P Q
   | _, _ => throwUnsupportedSyntax
